examples/store/proofs/client/close.v
@@ -34,12 +34,12 @@ Proof.
 iIntros "(_ & _ & _ & #?)".
 iIntros "!> %Φ client post".
 iDestruct "client" as "(conn & %db & ready & state)".
-iPoseProof (RPC.client_connected_keys with "conn") as "#[-> ->]".
+iPoseProof (RPC.client_connected_session with "conn") as "#sess".
 wp_lam. wp_pures.
 wp_apply (RPC.wp_close with "[$conn]"); eauto.
 iIntros "pub". iApply "post". iFrame. 
 iDestruct "ready" as "[#?|ready]"; eauto.
-iLeft. by iApply Conn.session_failed_failure.
+iLeft. by iApply session_compromised'.
 Qed.
 
 End Verif.
